



We can write the given equation of the circle in vector form as: 

$$(\mathbf{x}-\mathbf{c})^T(\mathbf{x}-\mathbf{c})=r^2,$$ 

where $\mathbf{c}=[a,b]$ and $r$ are the center and radius of the circle respectively. 

Let $\mathbf{u}=[a^2+b^2-r^2,1,1,0,-2a,-2b]^T$ be the given vector, and let $\mathbf{\phi}(\mathbf{x})$ be one of the transformations given in the choices. Then we need to find which transformation will result in 

$$\mathbf{\phi}(\mathbf{x})^T \mathbf{u} = 0$$ 

for all $\mathbf{x}=[x_1,x_2]$. 

We can check each transformation one by one: 

1. $\mathbf{\phi}_1(\mathbf{x}) = [1,x_1^2,x_2^2,x_1,x_2,x_1x_2]^T$

\begin{align*}
\mathbf{\phi}_1(\mathbf{x})^T \mathbf{u} &= [1,x_1^2,x_2^2,x_1,x_2,x_1x_2] \cdot [a^2+b^2-r^2,1,1,0,-2a,-2b]^T \\
&= (a^2+b^2-r^2) + x_1^2 - r^2 + x_2^2 - r^2 - 2ax_1 - 2bx_2 + 2abx_1x_2
\end{align*}

This is a quadratic function of $x_1$ and $x_2$, so it cannot be zero for all $\mathbf{x}$, unless it is identically zero. However, it is not identically zero, because the constant term $a^2+b^2-r^2-2r^2$ is not zero.

2. $\mathbf{\phi}_2(\mathbf{x}) = [\ x_1^2,\ x_2^2,\ x_1x_2,\ x_1,\ x_2,\ 1\ ]^T$

\begin{align*}
\mathbf{\phi}_2(\mathbf{x})^T \mathbf{u} &= [x_1^2,x_2^2,x_1x_2,x_1,x_2,1] \cdot [a^2+b^2-r^2,1,1,0,-2a,-2b]^T \\
&= a^2 x_1^2 + b^2 x_2^2 + 2abx_1x_2 - r^2 (x_1^2 + x_2^2) - 2ax_1 - 2bx_2 + a^2+b^2-r^2 \\
&= (a^2+b^2-r^2) + (a^2-r^2)x_1^2 + (b^2-r^2)x_2^2 - 2ax_1 - 2bx_2 + 2abx_1x_2
\end{align*}

This is again a quadratic function of $x_1$ and $x_2$, but now the coefficients of $x_1^2$ and $x_2^2$ are $(a^2-r^2)$ and $(
