![image](https://user-images.githubusercontent.com/89120960/232210743-2a762ad1-3b89-4acc-aab4-01539899e899.png)


<p>
  Formulations 2 and 3 are always equivalent.

To see why, let's first expand the inner maximization in Formulation-2 as:

max
⁡
�
≥
0
{
(
�
(
�
)
⋅
�
)
+
�
(
�
)
}
=
sup
⁡
�
≥
0
{
(
�
(
�
)
⋅
�
)
+
�
(
�
)
}
max 
α≥0
​
 {(g(w)⋅α)+f(w)}=sup 
α≥0
​
 {(g(w)⋅α)+f(w)}

Here, we have introduced a scalar variable $\alpha$ and used the fact that maximizing over non-negative scalars $\alpha$ is equivalent to taking their supremum.

Substituting this expression back into Formulation-2, we obtain:

min
⁡
�
{
sup
⁡
�
≥
0
{
(
�
(
�
)
⋅
�
)
+
�
(
�
)
}
}
min 
w
​
 {sup 
α≥0
​
 {(g(w)⋅α)+f(w)}}

Now, we can interchange the order of the minimization and supremum operations, which gives us Formulation-3:

max
⁡
�
≥
0
{
min
⁡
�
{
(
�
(
�
)
⋅
�
)
+
�
(
�
)
}
}
max 
α≥0
​
 {min 
w
​
 {(g(w)⋅α)+f(w)}}

Therefore, Formulation-2 and Formulation-3 are equivalent.

Formulation-1, on the other hand, is a different type of optimization problem that involves only a single constraint. In general, it is not equivalent to Formulation-2 or Formulation-3.






Regenerate response
  </p>
