![image](https://user-images.githubusercontent.com/89120960/232234311-537c6ea6-2707-406f-a775-c17e606810a9.png)


<p>
  Yes, I can help you derive the expression for the objective function of the dual.

Starting with the expression for the dual problem:

maximize
�
α
∈
R
n
−
1
2
∑
i
1
n
∑
j
1
n
α
i
α
j
y
i
y
j
x
i
T
x
j
,
subject to
�
i
α
i
0
and
0
≤
α
i
≤
C
.

The Lagrangian for this problem is given by:

L(α, λ) = 1/2 ∑i∑j αi αj yi yj xiTxj − ∑i λi αi + ∑i ξi(C − αi) − ∑i μi αi

Where λ, ξ and μ are Lagrange multipliers for the constraints.

Now, we need to derive the dual function by minimizing L(α, λ) with respect to α and then maximizing with respect to λ. Differentiating L(α, λ) with respect to α and setting it to zero, we get:

∑j yj αj xjTx i − λi − μi = 0

Rearranging this equation, we get:

αi = (λi − μi)/yi(x iTx i) − ∑j≠i αj yj(xjTx i)

Plugging this back into the Lagrangian, we get:

L(λ) = ∑i λi − 1/2 ∑i∑j λi λj yi yj xiTxj

css
Copy code
    − ∑i≠j λi λj yi yj xiTxj + ∑i ξi(C − (λi − μi)/yi(x iTx i) − ∑j≠i αj yj(xjTx i)) − ∑i μi (λi − μi)/yi(x iTx i) − ∑i λi
Simplifying and removing the terms that do not depend on λ, we get:

L(λ) = ∑i λi − 1/2 ∑i∑j λi λj yi yj xiTxj

css
Copy code
    − ∑i≠j λi λj yi yj xiTxj − 1/2 ∑i λi yi(xiTxi)−2 ∑i≠j λi yi yj(xiTxj)
This can be further simplified as:

L(λ) = ∑i λi − 1/2 ∑i∑j λi λj yi yj xiTxj

css
Copy code
    − ∑i≠j λi λj yi yj xiTxj − 1/2 ∑i λi yi(xiTxi)−2 ∑i≠j λi yi yj(xiTxj)

    = ∑i λi − 1/2 λT(YTX)(XY)λ
Therefore, the objective function of the dual has the form:

1/2 λT(YTX)(XY)λ - λT(1n) + c

where c is a constant term and 1n is a vector of ones with n elements. This can be rewritten as:

1 - 1/2 λT(1n) - 1/2 λT(YTX)(XY)λ

or

1/2 λT(YTX)(XY)λ - 1/2 λT(1n) + 1
</p>
