


<p>
  Sure, here's the formatted solution:

To show that the objective function of the dual has the form:

1
2
∑
�
=
1
�
∑
�
=
1
�
�
�
�
�
�
�
�
�
�
�
�
�
�
−
∑
�
=
1
�
�
�
2
1
​
  
i=1
∑
n
​
  
j=1
∑
n
​
 α 
i
​
 α 
j
​
 y 
i
​
 y 
j
​
 x 
i
T
​
 x 
j
​
 − 
i=1
∑
n
​
 α 
i
​
 
We start by substituting the definition of $X$ and $Y$:

1
2
∑
�
=
1
�
∑
�
=
1
�
�
�
�
�
�
�
�
�
(
�
�
�
�
�
+
1
)
2
−
∑
�
=
1
�
�
�
2
1
​
  
i=1
∑
n
​
  
j=1
∑
n
​
 α 
i
​
 α 
j
​
 y 
i
​
 y 
j
​
 (x 
i
T
​
 x 
j
​
 +1) 
2
 − 
i=1
∑
n
​
 α 
i
​
 
Expanding the squared term, we get:

1
2
∑
�
=
1
�
∑
�
=
1
�
�
�
�
�
�
�
�
�
(
�
�
�
�
�
)
2
+
�
�
�
�
�
�
�
�
�
�
�
�
�
+
�
�
�
�
�
�
�
�
−
∑
�
=
1
�
�
�
2
1
​
  
i=1
∑
n
​
  
j=1
∑
n
​
 α 
i
​
 α 
j
​
 y 
i
​
 y 
j
​
 (x 
i
T
​
 x 
j
​
 ) 
2
 +α 
i
​
 α 
j
​
 y 
i
​
 y 
j
​
 x 
i
T
​
 x 
j
​
 +α 
i
​
 α 
j
​
 y 
i
​
 y 
j
​
 − 
i=1
∑
n
​
 α 
i
​
 
The third term in the above equation is a constant and can be ignored when maximizing the dual objective. The first term is quadratic in $\alpha$ and the second term is linear in $\alpha$, so the objective function has the form:

−
1
2
�
�
�
�
+
�
�
�
− 
2
1
​
 α 
T
 Qα+p 
T
 α
where

�
�
�
=
�
�
�
�
(
�
�
�
�
�
)
2
,
�
�
=
−
1
Q 
ij
​
 =y 
i
​
 y 
j
​
 (x 
i
T
​
 x 
j
​
 ) 
2
 ,p 
i
​
 =−1
This is the form of the objective function we were asked to show.
</p>
